src/Util/Fin.v
@@ -17,6 +17,24 @@ end.
 
 Module NOptions.
 
+Fixpoint n_Somes {T : Set} n (x : T) : n_options n T :=
+match n as n' return n_options n' T with
+| 0 => x
+| S n => Some (n_Somes n x)
+end.
+
+Fixpoint sequence {T : Set -> Set} (pure : forall [A : Set], A -> T A)
+                  (bind : forall [A B : Set], (A -> T B) -> T A -> T B)
+                  {A n} (x : n_options n (T A)) : T (n_options n A) :=
+match n as n' return n_options n' (T A) -> T (n_options n' A) with
+| 0 => fun x => x
+| S n => fun x =>
+  match x with
+  | None => pure None
+  | Some x => bind (fun x => pure (Some x)) (sequence pure bind x)
+  end
+end x.
+
 Lemma sum_prop (n m : nat) {T} : n_options n (n_options m T) = n_options (n + m) T.
 Proof. induction n. auto. simpl. apply (f_equal (fun (T : Set) => option T)). apply IHn. Qed.
 
@@ -72,6 +90,23 @@ Qed.
 Lemma to_nat_rew n m (i : fin n) (p : n = m) : to_nat (rew [fin] p in i) = to_nat i.
 Proof. destruct p. auto. Qed.
 
+Lemma compare {n} (i j : fin n) : {to_nat i < to_nat j} + {i = j} + {to_nat i > to_nat j}.
+Proof.
+  induction n. inversion i. destruct i as [ i | ]; destruct j as [ j | ]; auto.
+  - edestruct IHn as [ [ lt | eq ] | gt ].
+    * left. left. apply le_n_S. apply lt.
+    * left. right. f_equal. auto.
+    * right. apply le_n_S. auto.
+  - right. apply Nat.lt_0_succ.
+  - left. left. apply Nat.lt_0_succ.
+Defined.
+
+Lemma eq_dec {n} (i j : fin n) : {i = j} + {i <> j}.
+Proof.
+  destruct (compare i j) as [ [ lt | eq ] | gt ]; auto.
+  all: right; intro; subst j; eapply Nat.lt_irrefl; eauto.
+Defined.
+
 Fixpoint of_nat n i (p : i < n) : fin n :=
 match n as n', p return fin n' with
 | 0, p => False_rec _ (match p with end)
@@ -116,6 +151,34 @@ Proof. auto. Qed.
 
 Lemma fin_0_0 {n m} (p : S n = S m) : rew [fin] p in (None : fin (S n)) = None.
 Proof. refine (match p with eq_refl => eq_refl end). Qed.
+
+Fixpoint of_n_options {T n} (x : n_options n T) : sum T (fin n) :=
+match n as n' return n_options n' T -> sum T (fin n') with
+| 0 => inl
+| S n => fun x =>
+  match x with
+  | None => inr None
+  | Some x =>
+    match of_n_options x with
+    | inl x => inl x
+    | inr x => inr (Some x)
+    end
+  end
+end x.
+
+Fixpoint to_n_options T {n} (i : fin n) : n_options n T :=
+match n as n' return fin n' -> n_options n' T with
+| 0 => fun i => match i with end
+| S n => fun i =>
+  match i with
+  | None => None
+  | Some i => Some (to_n_options T i)
+  end
+end i.
+
+Lemma fin_n_options_fin {n} (i : fin n) T : of_n_options (to_n_options T i) = inr i.
+Proof. induction n. inversion i. destruct i as [ i | ]; auto. simpl. rewrite IHn. auto. Qed.
+
 
 End Fin.
 
@@ -332,6 +395,35 @@ Corollary map_ext {T R : Set} [f g : T -> R] {n} (xs : vec T n)
                   : map f xs = map g xs.
 Proof. repeat rewrite map_prop. apply a2v_ext. auto. Qed.
 
+Fixpoint sequence {T : Set -> Set} (pure : forall [A : Set], A -> T A)
+                  (bind : forall [A B : Set], (A -> T B) -> T A -> T B)
+                  {A n} (xs : vec (T A) n) : T (vec A n) :=
+match xs in vec _ n' return T (vec A n') with
+| NilVec => pure NilVec
+| ConsVec x xs =>
+  bind (fun x =>
+    bind (fun xs =>
+      pure (ConsVec x xs)) (sequence pure bind xs)) x 
+end.
+
+Lemma sequence_pure {T : Set -> Set} (pure : forall [A : Set], A -> T A)
+                    (bind : forall [A B : Set], (A -> T B) -> T A -> T B)
+                    (bind_pure : forall (A B : Set) (k : A -> T B) (x : A), bind k (pure x) = k x)
+                    {A n} (xs : vec A n) : sequence pure bind (map (pure (A:=A)) xs) = pure xs.
+Proof. induction xs. auto. simpl. rewrite IHxs. rewrite bind_pure. rewrite bind_pure. auto. Qed.
+
+Lemma sequence_pure' {T : Set -> Set} (pure : forall [A : Set], A -> T A)
+                     (bind : forall [A B : Set], (A -> T B) -> T A -> T B)
+                     (bind_pure : forall (A B : Set) (k : A -> T B) (x : A), bind k (pure x) = k x)
+                     {A n} (xs : vec (T A) n) (ys : array A n)
+                     (H : forall i, Vec.v2a xs i = pure (ys i))
+                     : sequence pure bind xs = pure (Vec.a2v ys).
+Proof.
+  transitivity (sequence pure bind (Vec.map (pure _) (Vec.a2v ys))). f_equal. symmetry.
+  etransitivity. apply map_prop. etransitivity. apply a2v_ext. intro. rewrite array_vec_array.
+  symmetry. eauto. apply vec_array_vec. etransitivity. apply sequence_pure. auto. reflexivity.
+Qed.
+
 Definition indices n := a2v (fun (i : fin n) => i).
 
 Fixpoint to_list {T n} (xs : vec T n) : list T :=
@@ -352,5 +444,117 @@ match xs as xs' return vec T (length xs') with
 | nil => NilVec
 | cons x xs => ConsVec x (of_list xs)
 end.
+
+Fixpoint find {T : Set} [P : T -> Prop] (dec : forall x, {P x} + {~(P x)})
+              {n} (xs : vec T n) : option (fin n) :=
+match xs in vec _ n' return option (fin n') with
+| NilVec => None
+| ConsVec x xs =>
+  match dec x with
+  | left _ => Some None
+  | right _ =>
+    match find dec xs with
+    | None => None
+    | Some i => Some (Some i)
+    end
+  end
+end.
+
+Lemma find_p {T : Set} [P : T -> Prop] (dec : forall x, {P x} + {~(P x)})
+             {n} (xs : vec T n) (i : fin n) (H : find dec xs = Some i) : P (v2a xs i).
+Proof.
+  induction xs. inversion H. generalize dependent H. simpl. destruct (dec t).
+  - intro. inversion H. auto.
+  - destruct (find dec xs) as [ j | ]; intro; inversion H. apply IHxs. auto.
+Qed.
+
+Lemma find_not_p {T : Set} [P : T -> Prop] (dec : forall x, {P x} + {~(P x)})
+                 {n} (xs : vec T n) (H : find dec xs = None) : forall i, ~(P (v2a xs i)).
+Proof.
+  induction xs. intro. inversion i. generalize dependent H. simpl. destruct (dec t).
+  - intro. inversion H.
+  - destruct (find dec xs) as [ j | ]; intro. inversion H. intro. destruct i as [ i | ]; auto.
+Qed.
+
+Lemma find_some {T : Set} [P : T -> Prop] (dec : forall x, {P x} + {~(P x)})
+                {n} (xs : vec T n) (i : fin n) (H : P (v2a xs i))
+                : exists j, find dec xs = Some j.
+Proof.
+  remember (find dec xs) as res. destruct res as [ j | ]. eexists. reflexivity.
+  exfalso. eapply find_not_p. eauto. eauto.
+Qed.
+
+Lemma find_none {T : Set} [P : T -> Prop] (dec : forall x, {P x} + {~(P x)})
+                {n} (xs : vec T n) (H : forall i, ~(P (v2a xs i)))
+                : find dec xs = None.
+Proof.
+  remember (find dec xs) as res. destruct res as [ j | ]; auto.
+  exfalso. eapply H. eapply find_p. eauto.
+Qed.
+
+Definition is_distinct {T : Set} (P : T -> Prop) {n} (xs : vec T n) : Prop :=
+  forall i j, P (v2a xs i) -> P (v2a xs j) -> i = j.
+
+Lemma find_distinct_some {T : Set} [P : T -> Prop] (dec : forall x, {P x} + {~(P x)})
+                         {n} (xs : vec T n) (Hxs : is_distinct P xs)
+                         (i : fin n) (H : P (v2a xs i)) : find dec xs = Some i.
+Proof.
+  destruct (find_some dec xs i H) as [ j Hj ]. rewrite Hj.
+  f_equal. apply Hxs; eauto. eapply find_p. eauto.
+Qed.
+
+Lemma distinct_indices_len {n m} (xs : vec (fin n) m)
+                           (H : forall j, is_distinct (fun i => i = j) xs)
+                           : m <= n.
+Proof.
+  generalize dependent m. induction n; intros. destruct xs. auto. inversion f.
+  destruct xs. apply le_0_n. rename n0 into m. rename f into j. apply le_n_S. unshelve eapply IHn.
+  - apply Vec.a2v. intro i. remember (Vec.v2a xs i) as j'.
+    destruct (Fin.compare j' j) as [ [ lt | eq ] | gt ].
+    * unshelve eapply Fin.of_nat. apply (Fin.to_nat j'). eapply Nat.lt_le_trans. eauto.
+      apply le_S_n. apply Fin.to_nat_prop.
+    * subst j'. specialize (H j None (Some i) eq_refl eq). inversion H.
+    * unshelve eapply Fin.of_nat. apply (pred (Fin.to_nat j')). destruct j' as [ j' | ].
+      apply Fin.to_nat_prop. inversion gt.
+  - Opaque Fin.compare.
+    intro j'. intros i1 i2. repeat rewrite Vec.array_vec_array. simpl.
+    destruct (Fin.compare (v2a xs i1) j) as [ [ lt1 | eq1 ] | gt1 ];
+    destruct (Fin.compare (v2a xs i2) j) as [ [ lt2 | eq2 ] | gt2 ];
+    simpl; intros; subst j'; try apply Fin.of_nat_inj in H1.
+    4, 5, 6: set H as H'; specialize (H' j None (Some i1) eq_refl eq1); inversion H'.
+    2, 5: set H as H'; specialize (H' j None (Some i2) eq_refl eq2); inversion H'.
+    * apply (Fin.to_nat_inj (v2a xs i2)) in H1.
+      specialize (H (v2a xs i1) (Some i1) (Some i2) eq_refl H1). inversion H. auto.
+    * remember (v2a xs i2) as j2. destruct j2 as [ j2 | ].
+      specialize (H1 : Fin.to_nat j2 = Fin.to_nat (v2a xs i1)). rewrite <- H1 in lt1.
+      exfalso. apply (Nat.nle_succ_diag_l (Fin.to_nat j)). etransitivity; eauto.
+      exfalso. eapply (Nat.nlt_0_r). apply gt2.
+    * remember (v2a xs i1) as j1. destruct j1 as [ j1 | ].
+      specialize (H1 : Fin.to_nat (v2a xs i2) = Fin.to_nat j1). rewrite H1 in lt2.
+      exfalso. apply (Nat.nle_succ_diag_l (Fin.to_nat j)). etransitivity; eauto.
+      exfalso. eapply (Nat.nlt_0_r). apply gt1.
+    * remember (v2a xs i1) as j1. remember (v2a xs i2) as j2.
+      destruct j1 as [ j1 | ]. destruct j2 as [ j2 | ]. apply Fin.to_nat_inj in H1. subst j2.
+      specialize (H (Some j1) (Some i1) (Some i2) (eq_sym Heqj1) (eq_sym Heqj2)). inversion H. auto.
+      inversion gt2. inversion gt1.
+    Transparent Fin.compare.
+Qed.
+
+Definition is_permutation {n m} (xs : vec (fin n) m) :=
+  n = m /\ forall j, is_distinct (fun i => i = j) xs.
+
+Lemma all_in_permutation {n m} (xs : vec (fin n) m) j (H : is_permutation xs)
+                         : exists i, Vec.v2a xs i = j.
+Proof.
+  remember (find (fun i => Fin.eq_dec i j) xs) as res. symmetry in Heqres. destruct res as [ i | ].
+  - apply find_p in Heqres. eexists. eauto.
+  - assert (Hm : S m <= n).
+    * specialize (find_not_p _ xs Heqres). simpl. intro.
+      apply (distinct_indices_len (ConsVec j xs)). intro j'. intros i1 i2. intros.
+      destruct i1 as [ i1 | ]; destruct i2 as [ i2 | ]; auto.
+      destruct H. f_equal. eapply H3; eauto.
+      all: exfalso; subst j'; eapply H0; symmetry; eauto.
+    * exfalso. apply (Nat.lt_irrefl n). destruct H. subst m. auto.
+Qed.
 
 End Vec.
