src/Util/Misc.v
@@ -1,0 +1,19 @@
+
+
+Definition option_pure [A : Set] (x : A) : option A := Some x.
+
+Definition option_bind [A B : Set] (k : A -> option B) (x : option A) : option B :=
+  option_rec (fun _ => option B) k None x.
+
+Lemma option_bind_pure {A B : Set} (k : A -> option B) (x : A)
+                       : option_bind k (option_pure x) = k x.
+Proof. reflexivity. Qed.
+
+Lemma option_pure_bind {A B : Set} (k : A -> option B) (x : option A)
+                       : option_bind (option_pure (A:=A)) x = x.
+Proof. destruct x; reflexivity. Qed.
+
+Lemma option_bind_assoc {A B C : Set} (k1 : A -> option B) (k2 : B -> option C) (x : option A)
+                        : option_bind k2 (option_bind k1 x)
+                        = option_bind (fun x => option_bind k2 (k1 x)) x.
+Proof. destruct x; reflexivity. Qed.
